Auto/Embedding/LamThm.lean
@@ -2,22 +2,6 @@ import Auto.Embedding.LamBase
 
 namespace Auto.Embedding.Lam
 
-structure LamThmJudge where
-  lctx  : List LamSort
-  rterm : LamTerm
-  rty   : LamSort
-
-def LamThmWF (lval : LamValuation) (ltj : LamThmJudge) :=
-  ∀ (lctx' : Nat → LamSort), LamWF lval.ilVal.toLamTyVal ⟨pushLCtxs ltj.lctx lctx', ltj.rterm, ltj.rty⟩
-
-def LamThmWF.ofBVarLifts (lval : LamValuation) (ltj : LamThmJudge)
-  (hWF : LamThmWF lval ltj) : Nat := sorry
-
-def LamThmValid (lval : LamValuation) (lctx : List LamSort) (t : LamTerm) :=
-  ∀ (lctx' : Nat → LamSort) (lctxTerm : ∀ n, (pushLCtxs lctx lctx' n).interp lval.ilVal.tyVal),
-    ∃ (wf : LamWF lval.ilVal.toLamTyVal ⟨pushLCtxs lctx lctx', t, .base .prop⟩),
-      GLift.down (LamWF.interp lval (pushLCtxs lctx lctx') lctxTerm wf)
-
 def Eq.symm.WF (wf : LamWF ltv ⟨lctx, .app (.app (.base (.eq n)) a) b, .base .prop⟩) :
   LamWF ltv ⟨lctx, .app (.app (.base (.eq n)) b) a, .base .prop⟩ :=
   match wf with
